\documentclass{article}
\usepackage{cmap}					% поиск в PDF
\usepackage{mathtext} 				% русские буквы в формулах
\usepackage[T2A]{fontenc}			% кодировка
\usepackage[utf8]{inputenc}			% кодировка исходного текста
\usepackage[english,russian]{babel}	

\begin{document}

\section{Task}
\Large
Привести к нормальной форме $\lambda$-терм  \\
$
((\lambda a.(\lambda b.b\ b) \ (\lambda b.b\ b)) \ b) \ ((\lambda c.(c \ b)) \ (\lambda a.a))
$

\section{Solution}
\Large
$
((\lambda a.(\lambda b.b\ b) \ (\lambda b.b\ b)) \ b) \ ((\lambda c.(c \ b)) \ (\lambda a.a)) \\
\rightarrow _{\beta} 
((\lambda b.b\ b) \ (\lambda b.b\ b)) \ ((\lambda c.(c \ b)) \ (\lambda a.a)) \\
\rightarrow _{\beta} 
((\lambda b.b\ b) \ (\lambda b.b\ b)) \ ((\lambda a.a) \ b) \\
\rightarrow _{\beta} 
((\lambda b.b\ b) \ (\lambda b.b\ b)) \ b
\equiv \Omega \ b
$

\end{document}
